VCV-io/OracleComp/DistSemantics/Support.lean
@@ -10,10 +10,17 @@ namespace OracleComp
 
 variable {spec : OracleSpec} {α β : Type}
 
+/-- The `support` of a computation `oa` is the set of all possible output values,
+assuming that all output values of the oracles are possible.
+This is naturally compatible with `evalDist` where the oracles respond uniformly. -/
 def support : OracleComp spec α → Set α
 | pure' _ x => {x}
 | query_bind' _ _ _ oa => ⋃ u, (oa u).support
 
+/-- Given a `DecidableEq` instance on the return type, we can construct
+a `Finset` of possible outputs. Without this we can't remove duplicate values from
+the list of outputs being constructed. This also relies on the `DecidableEq` instances
+on `spec.range i` that are included in the definition of `OracleSpec`. -/
 def finSupport [DecidableEq α] : OracleComp spec α → Finset α
 | pure' _ x => {x}
 | query_bind' _ _ _ oa => Finset.biUnion Finset.univ (λ u ↦ (oa u).finSupport)
@@ -74,6 +81,7 @@ end basic
 
 section coe
 
+/-- `finSupport` when viewed as a `Set` gives the regular `support` of the computation.  -/
 @[simp] lemma coe_finSupport : {α : Type} → [DecidableEq α] →
   (oa : OracleComp spec α) → ↑oa.finSupport = oa.support
 | _, _, pure' _ x => by simp
